backend/Conventions.v
@@ -120,7 +120,6 @@ Definition agree_callee_save (ls1 ls2: Locmap.t) : Prop :=
 (** * Calling convention *)
 
 Require Import LanguageInterface.
-Require Import Invariant.
 Require Import CKLR.
 Require Import String.
 Require Import Values.
@@ -144,6 +143,8 @@ Canonical Structure li_locset: language_interface :=
   {|
     query := locset_query;
     reply := Locmap.t * mem;
+    query_is_internal ge q :=
+      Globalenvs.Senv.block_is_internal ge (lq_fb q);
   |}.
 
 Record match_locset_query (R: cklr) (w: world R) (q1 q2: locset_query) :=
@@ -155,12 +156,9 @@ Record match_locset_query (R: cklr) (w: world R) (q1 q2: locset_query) :=
   }.
 
 Definition cc_locset (R: cklr): callconv li_locset li_locset :=
-  {|
-    ccworld := world R;
-    match_senv := Events.symbols_inject @@ [mi R];
-    match_query := match_locset_query R;
-    match_reply := <> (- ==> Val.inject @@ [mi R]) * match_mem R;
-  |}.
+  cc_klr
+    (match_locset_query R)
+    (<> (- ==> Val.inject @@ [mi R]) * match_mem R).
 
 (** Triangular diagrams *)
 
@@ -171,12 +169,9 @@ Inductive match_locset_query_tr (R: cklr) (w: world R) q: locset_query -> Prop :
     match_locset_query_tr R w q q.
 
 Definition cc_locset_tr R: callconv li_locset li_locset :=
-  {|
-    ccworld := world R;
-    match_senv := Events.symbols_inject @@ [mi R];
-    match_query := match_locset_query_tr R;
-    match_reply := <> (- ==> Val.inject @@ [mi R]) * match_mem R;
-  |}.
+  cc_klr
+    (match_locset_query_tr R)
+    (<> (- ==> Val.inject @@ [mi R]) * match_mem R).
 
 (** We now define the calling convention between C and locset languages. *)
 
@@ -192,15 +187,14 @@ Inductive cc_alloc_mr: _ -> reply li_c -> reply li_locset -> Prop :=
     cc_alloc_mr (sg, rs) (res, m') (rs', m').
 
 Definition cc_alloc: callconv li_c li_locset :=
-  {|
-    ccworld := signature * Locmap.t;
-    match_senv w := eq;
-    match_query := cc_alloc_mq;
-    match_reply := cc_alloc_mr;
-  |}.
+  cc_klr
+    cc_alloc_mq
+    cc_alloc_mr.
 
+(*
 Definition alloc_sg (w: ccworld cc_alloc) := fst w.
 Definition alloc_rs (w: ccworld cc_alloc) := snd w.
+*)
 
 Lemma match_cc_alloc fb sg args rs m:
   args = map (fun p => Locmap.getpair p rs) (loc_arguments sg) ->
@@ -213,12 +207,13 @@ Lemma match_cc_alloc fb sg args rs m:
       m1' = m2'.
 Proof.
   intros Hargs.
-  exists (sg, rs). split.
+  exists (Some (sg, rs)). split.
   - constructor; eauto.
   - intros vres m1' rs' m2' Hr.
-    inv Hr. eauto.
+    inv Hr. inv H. eauto.
 Qed.
 
+(*
 Lemma match_query_cc_alloc (P: _ -> _ -> _ -> _ -> Prop):
   (forall id sg args rs m,
    args = map (fun p => Locmap.getpair p rs) (loc_arguments sg) ->
@@ -250,6 +245,7 @@ Ltac inv_alloc_query :=
   pattern (alloc_sg w), (alloc_rs w), q1, q2;
   revert w q1 q2 Hq;
   apply match_query_cc_alloc.
+*)
 
 (* XXX may be needed later
 Lemma locmap_setpair_getpair p ls l:
