games/AsmLinking.v
@@ -1,0 +1,167 @@
+Require Import LogicalRelations.
+Require Import Linking.
+Require Import GameSemantics.
+Require Import Composition.
+Require Import Values.
+Require Import LanguageInterface.
+Require Import AST.
+Require Import Globalenvs.
+Require Import Asm.
+Require Import RTS.
+Require Import ModuleSemantics.
+Require Import Smallstep.
+
+Definition asm p : modsem (li_asm -o li_asm) :=
+  Behavior.of (Asm.semantics p).
+
+Require Import Maps.
+Require Import List.
+
+Section HCOMP.
+  Context (p1 p2 p: Asm.program) (Hp: link p1 p2 = Some p).
+  Let L1 := Asm.semantics p1.
+  Let L2 := Asm.semantics p2.
+  Let L := Asm.semantics p.
+  Let L12 := HComp.semantics (symbolenv L) L1 L2.
+
+  Inductive res_state_rel {A B} (R : rel A B) : rel (@Res.state A) (@Res.state B) :=
+    | res_running_rel:
+        Monotonic Res.running (R ++> res_state_rel R)
+    | res_resumed_rel:
+        Monotonic Res.resumed (set_le R ++> res_state_rel R).
+
+  Inductive match_fc_states : rel FComp.state (state L) :=
+    | match_fc_states_l s1 :
+        match_fc_states
+          (FComp.running (inl s1) (FComp.inrk (initial_state L2)))
+          s1
+    | match_fc_states_r s2 :
+        match_fc_states
+          (FComp.running (inr s2) (FComp.inlk (initial_state L1)))
+          s2.
+
+  Inductive match_states : rel (state L12) (state L) :=
+    | match_states_running s s' :
+        match_fc_states s s' ->
+        match_states (Res.running s) s'
+    | match_states_resumed (S: FComp.state -> Prop) s' :
+        (forall s, S s -> match_fc_states s s') ->
+        match_states (Res.resumed S) s'.
+
+  Inductive link_cases : bool -> bool -> bool -> Prop :=
+    | lc_none : link_cases false false false
+    | lc_left : link_cases true false true
+    | lc_right : link_cases false true true.
+
+  Lemma query_is_internal_cases q:
+    link_cases
+      (query_is_internal li_asm (Genv.globalenv p1) q)
+      (query_is_internal li_asm (Genv.globalenv p2) q)
+      (query_is_internal li_asm (Genv.globalenv p) q).
+  Proof.
+  Admitted.
+
+  Lemma internal_hcomp_l q :
+    query_is_internal li_asm (Genv.globalenv p1) q = true ->
+    query_is_internal li_asm (Genv.globalenv p) q = true.
+  Admitted.
+
+  Lemma internal_hcomp_r q :
+    query_is_internal li_asm (Genv.globalenv p2) q = true ->
+    query_is_internal li_asm (Genv.globalenv p) q = true.
+  Admitted.
+
+  Lemma internal_hcomp_inv q :
+    query_is_internal li_asm (Genv.globalenv p) q = true ->
+    query_is_internal li_asm (Genv.globalenv p2) q = true \/
+    query_is_internal li_asm (Genv.globalenv p2) q = true.
+  Admitted.
+
+  Lemma asm_hcomp_fsim_cont_l :
+    fsim_match_cont cc_id (fun _ => match_states) tt
+      (Res.liftk (FComp.liftk (FComp.inlk (initial_state L1))
+                              (FComp.inrk (initial_state L2))))
+      (simple_initial_state Asm.initial_state (Genv.globalenv p)).
+  Proof.
+    intros [] [[] | q] _ [].
+    unfold Res.liftk, FComp.liftk, FComp.inlk, FComp.inrk.
+    cbn -[query_is_internal]. unfold simple_dom.
+    destruct (query_is_internal_cases q); constructor;
+    intros _ [_ [s Hs]]; inversion Hs as [x]; clear Hs; subst;
+    exists x; split; auto; repeat constructor.
+  Qed.
+
+  Lemma asm_hcomp_fsim_cont_r :
+    fsim_match_cont cc_id (fun _ => match_states) tt
+      (Res.liftk (FComp.liftk (FComp.inrk (initial_state L2))
+                              (FComp.inlk (initial_state L1))))
+      (simple_initial_state Asm.initial_state (Genv.globalenv p)).
+  Proof.
+    intros [] [[] | q] _ [].
+    unfold Res.liftk, FComp.liftk, FComp.inlk, FComp.inrk.
+    cbn -[query_is_internal]. unfold simple_dom.
+    destruct (query_is_internal_cases q); constructor;
+    intros _ [_ [s Hs]]; inversion Hs as [x]; clear Hs; subst;
+    exists x; split; auto; repeat constructor.
+  Qed.
+
+  Axiom external_call_empty :
+    forall ef ge vargs m t vres m',
+      ~ Events.external_call ef ge vargs m t vres m'.
+
+  Lemma asm_hcomp_fsim :
+    forward_simulation cc_id (HComp.semantics (symbolenv L) L1 L2) L.
+  Proof.
+    apply forward_simulation_step with (fun _ => match_states); simpl.
+    - reflexivity.
+    - apply asm_hcomp_fsim_cont_l.
+    - intros _ s12 s r12 k12 Hs H;
+      destruct H as  [s12 r12 k12 Hk12 Hr];
+      destruct Hk12 as [si r ki kj Hki | si r ki kj Hki];
+      destruct Hki as [si Hsi];
+      inversion Hs; clear Hs; subst;
+      inversion H0; clear H0; subst;
+      exists tt, (inl s), (simple_initial_state Asm.initial_state (Genv.globalenv p));
+      intuition auto using asm_hcomp_fsim_cont_l, asm_hcomp_fsim_cont_r;
+      constructor;
+      simpl in Hr; unfold FComp.liftk, FComp.inlk, FComp.inrk in Hr;
+      unfold simple_initial_state, simple_dom in Hr;
+      destruct (query_is_internal_cases s); simpl in Hr; try congruence.
+    - intros _ s12 t s12' Hs12' s Hs.
+      destruct Hs12' as [s12 t s12' Hs12' | s12 r12 k12 S12 Hk12 Hq | ].
+      + (* internal step *)
+        destruct Hs12' as  [si t si' kj Hsi' | si t si' kj Hsi']; simpl in *.
+      * inversion Hs; clear Hs; subst.
+        destruct Hsi'.
+        -- admit.
+        -- admit.
+        -- eelim external_call_empty; eauto.
+      * admit.
+      + (* internal switching *) 
+        simpl in *.
+        destruct Hk12 as [si r ki k' Hki | si r ki k' Hki]; simpl in *.
+      * destruct Hki as [si Hsi]; cbn -[li_asm] in Hq.
+        inversion Hs; clear Hs; subst.
+        inversion H0; clear H0; subst.
+        unfold FComp.liftk in Hq.
+        unfold FComp.inlk at 1, FComp.inrk at 1 3 in Hq.
+        unfold simple_initial_state at 1 2 4, simple_dom in Hq.
+        destruct (query_is_internal_cases s); simpl in Hq; try congruence.
+        inversion Hq; clear Hq; subst.
+        exists s. split.
+        -- admit. (* measured simulation *)
+        -- constructor.
+           intros x [y [z Hz]].
+           destruct Hz.
+           constructor.
+      * admit.
+      + (* resuming after internal switching *)
+        inversion Hs; clear Hs; subst.
+        specialize (H1 s0 H).
+        exists s. split.
+        -- admit. (* measured simulation *)
+        -- constructor; auto.
+        (* Need measured simulation -- can use whether internal matches
+                  currently executing component as measure *)
+  Admitted.
+End HCOMP.
